update preuve blocking semantic 5

examples/hoare_logic/blocking_semantics5/blocking_semantics5_HoareLogic_assert_rule_ext_1.v
@@ -236,136 +236,6 @@ Definition reductible(sigma:(map mident value)) (pi:(list (ident*
   sigma' pi' s').
 
 (* Why3 assumption *)
-Definition type_value(v:value): datatype :=
-  match v with
-  | Vvoid => TYunit
-  | (Vint int) => TYint
-  | (Vbool bool1) => TYbool
-  end.
-
-(* Why3 assumption *)
-Inductive type_operator : operator -> datatype -> datatype
-  -> datatype -> Prop :=
-  | Type_plus : (type_operator Oplus TYint TYint TYint)
-  | Type_minus : (type_operator Ominus TYint TYint TYint)
-  | Type_mult : (type_operator Omult TYint TYint TYint)
-  | Type_le : (type_operator Ole TYint TYint TYbool).
-
-(* Why3 assumption *)
-Definition type_stack  := (list (ident* datatype)%type).
-
-Parameter get_vartype: ident -> (list (ident* datatype)%type) -> datatype.
-
-Axiom get_vartype_def : forall (i:ident) (pi:(list (ident* datatype)%type)),
-  match pi with
-  | Nil => ((get_vartype i pi) = TYunit)
-  | (Cons (x, ty) r) => ((x = i) -> ((get_vartype i pi) = ty)) /\
-      ((~ (x = i)) -> ((get_vartype i pi) = (get_vartype i r)))
-  end.
-
-(* Why3 assumption *)
-Definition type_env  := (map mident datatype).
-
-(* Why3 assumption *)
-Inductive type_term : (map mident datatype) -> (list (ident* datatype)%type)
-  -> term -> datatype -> Prop :=
-  | Type_value : forall (sigma:(map mident datatype)) (pi:(list (ident*
-      datatype)%type)) (v:value), (type_term sigma pi (Tvalue v)
-      (type_value v))
-  | Type_var : forall (sigma:(map mident datatype)) (pi:(list (ident*
-      datatype)%type)) (v:ident) (ty:datatype), ((get_vartype v pi) = ty) ->
-      (type_term sigma pi (Tvar v) ty)
-  | Type_deref : forall (sigma:(map mident datatype)) (pi:(list (ident*
-      datatype)%type)) (v:mident) (ty:datatype), ((get sigma v) = ty) ->
-      (type_term sigma pi (Tderef v) ty)
-  | Type_bin : forall (sigma:(map mident datatype)) (pi:(list (ident*
-      datatype)%type)) (t1:term) (t2:term) (op:operator) (ty1:datatype)
-      (ty2:datatype) (ty:datatype), (type_term sigma pi t1 ty1) ->
-      ((type_term sigma pi t2 ty2) -> ((type_operator op ty1 ty2 ty) ->
-      (type_term sigma pi (Tbin t1 op t2) ty))).
-
-(* Why3 assumption *)
-Inductive type_fmla : (map mident datatype) -> (list (ident* datatype)%type)
-  -> fmla -> Prop :=
-  | Type_term : forall (sigma:(map mident datatype)) (pi:(list (ident*
-      datatype)%type)) (t:term), (type_term sigma pi t TYbool) ->
-      (type_fmla sigma pi (Fterm t))
-  | Type_conj : forall (sigma:(map mident datatype)) (pi:(list (ident*
-      datatype)%type)) (f1:fmla) (f2:fmla), (type_fmla sigma pi f1) ->
-      ((type_fmla sigma pi f2) -> (type_fmla sigma pi (Fand f1 f2)))
-  | Type_neg : forall (sigma:(map mident datatype)) (pi:(list (ident*
-      datatype)%type)) (f:fmla), (type_fmla sigma pi f) -> (type_fmla sigma
-      pi (Fnot f))
-  | Type_implies : forall (sigma:(map mident datatype)) (pi:(list (ident*
-      datatype)%type)) (f1:fmla) (f2:fmla), (type_fmla sigma pi f1) ->
-      ((type_fmla sigma pi f2) -> (type_fmla sigma pi (Fimplies f1 f2)))
-  | Type_let : forall (sigma:(map mident datatype)) (pi:(list (ident*
-      datatype)%type)) (x:ident) (t:term) (f:fmla) (ty:datatype),
-      (type_term sigma pi t ty) -> ((type_fmla sigma (Cons (x, ty) pi) f) ->
-      (type_fmla sigma pi (Flet x t f)))
-  | Type_forall1 : forall (sigma:(map mident datatype)) (pi:(list (ident*
-      datatype)%type)) (x:ident) (f:fmla), (type_fmla sigma (Cons (x, TYint)
-      pi) f) -> (type_fmla sigma pi (Fforall x TYint f))
-  | Type_forall2 : forall (sigma:(map mident datatype)) (pi:(list (ident*
-      datatype)%type)) (x:ident) (f:fmla), (type_fmla sigma (Cons (x, TYbool)
-      pi) f) -> (type_fmla sigma pi (Fforall x TYbool f))
-  | Type_forall3 : forall (sigma:(map mident datatype)) (pi:(list (ident*
-      datatype)%type)) (x:ident) (f:fmla), (type_fmla sigma (Cons (x, TYunit)
-      pi) f) -> (type_fmla sigma pi (Fforall x TYunit f)).
-
-(* Why3 assumption *)
-Inductive type_stmt : (map mident datatype) -> (list (ident* datatype)%type)
-  -> stmt -> Prop :=
-  | Type_skip : forall (sigma:(map mident datatype)) (pi:(list (ident*
-      datatype)%type)), (type_stmt sigma pi Sskip)
-  | Type_seq : forall (sigma:(map mident datatype)) (pi:(list (ident*
-      datatype)%type)) (s1:stmt) (s2:stmt), (type_stmt sigma pi s1) ->
-      ((type_stmt sigma pi s2) -> (type_stmt sigma pi (Sseq s1 s2)))
-  | Type_assigns : forall (sigma:(map mident datatype)) (pi:(list (ident*
-      datatype)%type)) (x:mident) (t:term) (ty:datatype), ((get sigma
-      x) = ty) -> ((type_term sigma pi t ty) -> (type_stmt sigma pi
-      (Sassign x t)))
-  | Type_if : forall (sigma:(map mident datatype)) (pi:(list (ident*
-      datatype)%type)) (t:term) (s1:stmt) (s2:stmt), (type_term sigma pi t
-      TYbool) -> ((type_stmt sigma pi s1) -> ((type_stmt sigma pi s2) ->
-      (type_stmt sigma pi (Sif t s1 s2))))
-  | Type_assert : forall (sigma:(map mident datatype)) (pi:(list (ident*
-      datatype)%type)) (p:fmla), (type_fmla sigma pi p) -> (type_stmt sigma
-      pi (Sassert p))
-  | Type_while : forall (sigma:(map mident datatype)) (pi:(list (ident*
-      datatype)%type)) (guard:term) (body:stmt) (inv:fmla), (type_fmla sigma
-      pi inv) -> ((type_term sigma pi guard TYbool) -> ((type_stmt sigma pi
-      body) -> (type_stmt sigma pi (Swhile guard inv body)))).
-
-Axiom type_inversion : forall (v:value),
-  match (type_value v) with
-  | TYbool => exists b:bool, (v = (Vbool b))
-  | TYint => exists n:Z, (v = (Vint n))
-  | TYunit => (v = Vvoid)
-  end.
-
-(* Why3 assumption *)
-Definition compatible_env(sigma:(map mident value)) (sigmat:(map mident
-  datatype)) (pi:(list (ident* value)%type)) (pit:(list (ident*
-  datatype)%type)): Prop := (forall (id:mident), ((type_value (get sigma
-  id)) = (get sigmat id))) /\ forall (id:ident), ((type_value (get_stack id
-  pi)) = (get_vartype id pit)).
-
-Axiom eval_type_term : forall (t:term) (sigma:(map mident value)) (pi:(list
-  (ident* value)%type)) (sigmat:(map mident datatype)) (pit:(list (ident*
-  datatype)%type)) (ty:datatype), (compatible_env sigma sigmat pi pit) ->
-  ((type_term sigmat pit t ty) -> ((type_value (eval_term sigma pi
-  t)) = ty)).
-
-Axiom type_preservation : forall (s1:stmt) (s2:stmt) (sigma1:(map mident
-  value)) (sigma2:(map mident value)) (pi1:(list (ident* value)%type))
-  (pi2:(list (ident* value)%type)) (sigmat:(map mident datatype)) (pit:(list
-  (ident* datatype)%type)), ((type_stmt sigmat pit s1) /\
-  ((compatible_env sigma1 sigmat pi1 pit) /\ (one_step sigma1 pi1 s1 sigma2
-  pi2 s2))) -> ((type_stmt sigmat pit s2) /\ (compatible_env sigma2 sigmat
-  pi2 pit)).
-
-(* Why3 assumption *)
 Fixpoint infix_plpl {a:Type} {a_WT:WhyType a}(l1:(list a)) (l2:(list
   a)) {struct l1}: (list a) :=
   match l1 with
@@ -486,94 +356,59 @@ Axiom eval_change_free : forall (f:fmla) (id:ident) (v:value),
   value)%type)), (eval_fmla sigma (Cons (id, v) pi) f) <-> (eval_fmla sigma
   pi f).
 
-Parameter fresh_from: fmla -> ident.
-
-Axiom fresh_from_fmla : forall (f:fmla), (fresh_in_fmla (fresh_from f) f).
-
-Parameter abstract_effects: stmt -> fmla -> fmla.
-
-Axiom abstract_effects_generalize : forall (sigma:(map mident value))
-  (pi:(list (ident* value)%type)) (s:stmt) (f:fmla), (eval_fmla sigma pi
-  (abstract_effects s f)) -> (eval_fmla sigma pi f).
-
-Axiom abstract_effects_monotonic : forall (s:stmt) (p:fmla) (q:fmla),
-  (valid_fmla (Fimplies p q)) -> forall (sigma:(map mident value)) (pi:(list
-  (ident* value)%type)), (eval_fmla sigma pi (abstract_effects s p)) ->
-  (eval_fmla sigma pi (abstract_effects s q)).
-
-Axiom abstract_effects_distrib_conj : forall (s:stmt) (p:fmla) (q:fmla)
-  (sigma:(map mident value)) (pi:(list (ident* value)%type)),
-  ((eval_fmla sigma pi (abstract_effects s p)) /\ (eval_fmla sigma pi
-  (abstract_effects s q))) -> (eval_fmla sigma pi (abstract_effects s (Fand p
-  q))).
+Axiom many_steps_seq : forall (sigma1:(map mident value)) (sigma3:(map mident
+  value)) (pi1:(list (ident* value)%type)) (pi3:(list (ident* value)%type))
+  (s1:stmt) (s2:stmt) (n:Z), (many_steps sigma1 pi1 (Sseq s1 s2) sigma3 pi3
+  Sskip n) -> exists sigma2:(map mident value), exists pi2:(list (ident*
+  value)%type), exists n1:Z, exists n2:Z, (many_steps sigma1 pi1 s1 sigma2
+  pi2 Sskip n1) /\ ((many_steps sigma2 pi2 s2 sigma3 pi3 Sskip n2) /\
+  (n = ((1%Z + n1)%Z + n2)%Z)).
 
 (* Why3 assumption *)
-Fixpoint wp(s:stmt) (q:fmla) {struct s}: fmla :=
-  match s with
-  | Sskip => q
-  | (Sassert f) => (Fand f (Fimplies f q))
-  | (Sseq s1 s2) => (wp s1 (wp s2 q))
-  | (Sassign x t) => let id := (fresh_from q) in (Flet id t (msubst q x id))
-  | (Sif t s1 s2) => (Fand (Fimplies (Fterm t) (wp s1 q))
-      (Fimplies (Fnot (Fterm t)) (wp s2 q)))
-  | (Swhile cond inv body) => (Fand inv (abstract_effects body
-      (Fand (Fimplies (Fand (Fterm cond) inv) (wp body inv))
-      (Fimplies (Fand (Fnot (Fterm cond)) inv) q))))
-  end.
+Definition valid_triple(p:fmla) (s:stmt) (q:fmla): Prop := forall (sigma:(map
+  mident value)) (pi:(list (ident* value)%type)), (eval_fmla sigma pi p) ->
+  forall (sigma':(map mident value)) (pi':(list (ident* value)%type)) (n:Z),
+  (many_steps sigma pi s sigma' pi' Sskip n) -> (eval_fmla sigma' pi' q).
 
-Axiom abstract_effects_writes : forall (sigma:(map mident value)) (pi:(list
-  (ident* value)%type)) (s:stmt) (q:fmla), (eval_fmla sigma pi
-  (abstract_effects s q)) -> (eval_fmla sigma pi (wp s (abstract_effects s
-  q))).
+(* Why3 assumption *)
+Definition total_valid_triple(p:fmla) (s:stmt) (q:fmla): Prop :=
+  forall (sigma:(map mident value)) (pi:(list (ident* value)%type)),
+  (eval_fmla sigma pi p) -> exists sigma':(map mident value),
+  exists pi':(list (ident* value)%type), exists n:Z, (many_steps sigma pi s
+  sigma' pi' Sskip n) /\ (eval_fmla sigma' pi' q).
 
-Axiom monotonicity : forall (s:stmt) (p:fmla) (q:fmla),
-  (valid_fmla (Fimplies p q)) -> (valid_fmla (Fimplies (wp s p) (wp s q))).
+Axiom consequence_rule : forall (p:fmla) (p':fmla) (q:fmla) (q':fmla)
+  (s:stmt), (valid_fmla (Fimplies p' p)) -> ((valid_triple p s q) ->
+  ((valid_fmla (Fimplies q q')) -> (valid_triple p' s q'))).
 
-Axiom distrib_conj : forall (s:stmt) (sigma:(map mident value)) (pi:(list
-  (ident* value)%type)) (p:fmla) (q:fmla), ((eval_fmla sigma pi (wp s p)) /\
-  (eval_fmla sigma pi (wp s q))) -> (eval_fmla sigma pi (wp s (Fand p q))).
+Axiom skip_rule : forall (q:fmla), (valid_triple q Sskip q).
 
-Axiom wp_reduction : forall (sigma:(map mident value)) (sigma':(map mident
-  value)) (pi:(list (ident* value)%type)) (pi':(list (ident* value)%type))
-  (s:stmt) (s':stmt), (one_step sigma pi s sigma' pi' s') -> forall (q:fmla),
-  (eval_fmla sigma pi (wp s q)) -> (eval_fmla sigma' pi' (wp s' q)).
+Axiom assign_rule : forall (p:fmla) (x:mident) (id:ident) (t:term),
+  (fresh_in_fmla id p) -> (valid_triple (Flet id t (msubst p x id))
+  (Sassign x t) p).
+
+Axiom seq_rule : forall (p:fmla) (q:fmla) (r:fmla) (s1:stmt) (s2:stmt),
+  ((valid_triple p s1 r) /\ (valid_triple r s2 q)) -> (valid_triple p
+  (Sseq s1 s2) q).
+
+Axiom if_rule : forall (t:term) (p:fmla) (q:fmla) (s1:stmt) (s2:stmt),
+  ((valid_triple (Fand p (Fterm t)) s1 q) /\ (valid_triple (Fand p
+  (Fnot (Fterm t))) s2 q)) -> (valid_triple p (Sif t s1 s2) q).
+
+Axiom assert_rule : forall (f:fmla) (p:fmla), (valid_fmla (Fimplies p f)) ->
+  (valid_triple p (Sassert f) p).
 
 (* Why3 goal *)
-Theorem progress : forall (s:stmt),
-  match s with
-  | Sskip => True
-  | (Sassign m t) => True
-  | (Sseq s1 s2) => True
-  | (Sif t s1 s2) => (forall (sigma:(map mident value)) (pi:(list (ident*
-      value)%type)) (sigmat:(map mident datatype)) (pit:(list (ident*
-      datatype)%type)) (q:fmla), (compatible_env sigma sigmat pi pit) ->
-      ((type_stmt sigmat pit s2) -> ((eval_fmla sigma pi (wp s2 q)) ->
-      ((~ (s2 = Sskip)) -> (reductible sigma pi s2))))) ->
-      ((forall (sigma:(map mident value)) (pi:(list (ident* value)%type))
-      (sigmat:(map mident datatype)) (pit:(list (ident* datatype)%type))
-      (q:fmla), (compatible_env sigma sigmat pi pit) -> ((type_stmt sigmat
-      pit s1) -> ((eval_fmla sigma pi (wp s1 q)) -> ((~ (s1 = Sskip)) ->
-      (reductible sigma pi s1))))) -> forall (sigma:(map mident value))
-      (pi:(list (ident* value)%type)) (sigmat:(map mident datatype))
-      (pit:(list (ident* datatype)%type)) (q:fmla), (compatible_env sigma
-      sigmat pi pit) -> ((type_stmt sigmat pit s) -> ((eval_fmla sigma pi
-      (wp s q)) -> ((~ (s = Sskip)) -> (reductible sigma pi s)))))
-  | (Sassert f) => True
-  | (Swhile t f s1) => True
-  end.
-destruct s; auto.
+Theorem assert_rule_ext : forall (f:fmla) (p:fmla), (valid_triple (Fimplies f
+  p) (Sassert f) p).
+unfold valid_triple.
+intros f p.
 intros.
-inversion H2; subst; clear H2.
-unfold reductible.
-apply eval_type_term with (sigma := sigma) (pi := pi) in H10 ; auto.
-assert (eval_term sigma pi t = Vbool true \/ 
-        eval_term sigma pi t = Vbool false).
-admit.
-destruct H2.
-do 3 eexists.
-apply one_step_if_true; auto.
-do 3 eexists.
-apply one_step_if_false; auto.
+inversion H0; subst; clear H0.
+simpl in H.
+inversion H1; subst; clear H1.
+inversion H2; subst; clear H2; auto.
+inversion H0.
 Qed.
 
 
