examples/hoare_logic/blocking_semantics3/blocking_semantics3_HoareLogic_assert_rule_ext_1.v
@@ -579,5 +579,3 @@ inversion H1; subst; clear H1.
 inversion H2; subst; clear H2; auto.
 inversion H0.
 Qed.
-
-
